@prefix : <http://www.semanticweb.org/thoma/ontologies/2020/10/untitled-ontology-19#> .
@prefix owl: <http://www.w3.org/2002/07/owl#> .
@prefix rdf: <http://www.w3.org/1999/02/22-rdf-syntax-ns#> .
@prefix xml: <http://www.w3.org/XML/1998/namespace> .
@prefix xsd: <http://www.w3.org/2001/XMLSchema#> .
@prefix rdfs: <http://www.w3.org/2000/01/rdf-schema#> .
@base <http://www.semanticweb.org/thoma/ontologies/2020/10/untitled-ontology-19> .

<http://www.semanticweb.org/thoma/ontologies/2020/10/untitled-ontology-19> rdf:type owl:Ontology .

#################################################################
#    Annotation properties
#################################################################

###  http://purl.org/dc/elements/1.1/date
<http://purl.org/dc/elements/1.1/date> rdf:type owl:AnnotationProperty .


###  http://purl.org/dc/elements/1.1/description
<http://purl.org/dc/elements/1.1/description> rdf:type owl:AnnotationProperty .


###  http://purl.org/dc/elements/1.1/title
<http://purl.org/dc/elements/1.1/title> rdf:type owl:AnnotationProperty .


###  http://www.w3.org/2003/01/geo/wgs84_pos#alt
<http://www.w3.org/2003/01/geo/wgs84_pos#alt> rdf:type owl:AnnotationProperty ;
                                              rdfs:comment """The WGS84 altitude of a SpatialThing (decimal meters 
above the local reference ellipsoid).""" ;
                                              rdfs:label "altitude" ;
                                              rdfs:domain <http://www.w3.org/2003/01/geo/wgs84_pos#SpatialThing> .


###  http://www.w3.org/2003/01/geo/wgs84_pos#lat
<http://www.w3.org/2003/01/geo/wgs84_pos#lat> rdf:type owl:AnnotationProperty ;
                                              rdfs:comment "The WGS84 latitude of a SpatialThing (decimal degrees)." ;
                                              rdfs:label "latitude" ;
                                              rdfs:domain <http://www.w3.org/2003/01/geo/wgs84_pos#SpatialThing> .


###  http://www.w3.org/2003/01/geo/wgs84_pos#location
<http://www.w3.org/2003/01/geo/wgs84_pos#location> rdf:type owl:AnnotationProperty ;
                                                   rdfs:subPropertyOf <http://xmlns.com/foaf/0.1/based_near> ;
                                                   rdfs:range <http://www.w3.org/2003/01/geo/wgs84_pos#SpatialThing> .


###  http://www.w3.org/2003/01/geo/wgs84_pos#long
<http://www.w3.org/2003/01/geo/wgs84_pos#long> rdf:type owl:AnnotationProperty ;
                                               rdfs:comment "The WGS84 longitude of a SpatialThing (decimal degrees)." ;
                                               rdfs:label "longitude" ;
                                               rdfs:domain <http://www.w3.org/2003/01/geo/wgs84_pos#SpatialThing> .


###  http://xmlns.com/foaf/0.1/based_near
<http://xmlns.com/foaf/0.1/based_near> rdf:type owl:AnnotationProperty .


#################################################################
#    Object Properties
#################################################################

###  http://www.semanticweb.org/thoma/ontologies/2020/10/untitled-ontology-19#aCommune
:aCommune rdf:type owl:ObjectProperty ;
          rdfs:subPropertyOf owl:topObjectProperty ;
          owl:inverseOf :aLieu ;
          rdfs:domain :Etablissement ,
                      :LieuTourisme ;
          rdfs:comment "Relie un lieu à une commune." .


###  http://www.semanticweb.org/thoma/ontologies/2020/10/untitled-ontology-19#aLieu
:aLieu rdf:type owl:ObjectProperty ;
       rdfs:domain :Commune ;
       rdfs:range :Etablissement ,
                  :LieuTourisme ;
       rdfs:comment "Relie une commune à un des lieux présents dans cette commune." .


#################################################################
#    Data properties
#################################################################

###  http://www.semanticweb.org/thoma/ontologies/2020/10/untitled-ontology-19#aAdresse
:aAdresse rdf:type owl:DatatypeProperty ;
          rdfs:domain :Etablissement ;
          rdfs:range xsd:string ;
          rdfs:comment "Relie un établissement à son adresse." .


###  http://www.semanticweb.org/thoma/ontologies/2020/10/untitled-ontology-19#aCodePostal
:aCodePostal rdf:type owl:DatatypeProperty ;
             rdfs:domain :Commune ,
                         :Etablissement ;
             rdfs:range xsd:integer ;
             rdfs:comment "Relie un lieu à son code postal." .


###  http://www.semanticweb.org/thoma/ontologies/2020/10/untitled-ontology-19#aDenivele
:aDenivele rdf:type owl:DatatypeProperty ;
           rdfs:domain :Randonnee ;
           rdfs:range xsd:double ;
           rdfs:comment "Indique le dénivelé d'une randonnée." .


###  http://www.semanticweb.org/thoma/ontologies/2020/10/untitled-ontology-19#aDistance
:aDistance rdf:type owl:DatatypeProperty ;
           rdfs:domain :Randonnee ;
           rdfs:range xsd:double ;
           rdfs:comment "Indique la distance à parcourir pour réaliser une randonnée." .


###  http://www.semanticweb.org/thoma/ontologies/2020/10/untitled-ontology-19#aDuree
:aDuree rdf:type owl:DatatypeProperty ;
        rdfs:domain :Randonnee ;
        rdfs:range xsd:integer ;
        rdfs:comment "Indique la durée estimée d'une randonnée." .


###  http://www.semanticweb.org/thoma/ontologies/2020/10/untitled-ontology-19#accessibleMobiliteReduite
:accessibleMobiliteReduite rdf:type owl:DatatypeProperty ;
                           rdfs:domain :LieuRemarquable ;
                           rdfs:range xsd:string ;
                           rdfs:comment """Précise si un lieu est accessible aux personnes à mobilité réduite.
A l'heure actuelle, nous ne connaissons cette information que pour les éléments de la classe LieuRemarquable.""" .


###  http://www.semanticweb.org/thoma/ontologies/2020/10/untitled-ontology-19#lat
:lat rdf:type owl:DatatypeProperty ;
     rdfs:domain <http://www.w3.org/2003/01/geo/wgs84_pos#SpatialThing> ;
     rdfs:range xsd:double ;
     rdfs:comment "Précise la latitude d'un élément de la classe SpatialThing." .


###  http://www.semanticweb.org/thoma/ontologies/2020/10/untitled-ontology-19#long
:long rdf:type owl:DatatypeProperty ;
      rdfs:domain <http://www.w3.org/2003/01/geo/wgs84_pos#SpatialThing> ;
      rdfs:range xsd:double ;
      rdfs:comment "Précise la longitude d'un élément de la classe SpatialThing." .


#################################################################
#    Classes
#################################################################

###  http://www.semanticweb.org/thoma/ontologies/2020/10/untitled-ontology-19#ArretTransport
:ArretTransport rdf:type owl:Class ;
                rdfs:subClassOf <http://www.w3.org/2003/01/geo/wgs84_pos#SpatialThing> ;
                rdfs:comment "Regroupe l'ensemble des arrets de transport. Il peut s'agir de tout type de transport : avion, bus, train, bateau, ..."@fr .


###  http://www.semanticweb.org/thoma/ontologies/2020/10/untitled-ontology-19#Centres_Hospitaliers
:Centres_Hospitaliers rdf:type owl:Class ;
                      rdfs:subClassOf :EtablissementSante ;
                      rdfs:comment """Regroupe l'ensemble des centres hospitaliers de la Réunion.
Il peut s'agir de centres hospitaliers réionaux, universitaires, ..."""@fr .


###  http://www.semanticweb.org/thoma/ontologies/2020/10/untitled-ontology-19#Commune
:Commune rdf:type owl:Class ;
         rdfs:subClassOf <http://www.w3.org/2003/01/geo/wgs84_pos#SpatialThing> ;
         rdfs:comment "Regroupe l'ensemble des communes."@fr .


###  http://www.semanticweb.org/thoma/ontologies/2020/10/untitled-ontology-19#Etablissement
:Etablissement rdf:type owl:Class ;
               rdfs:subClassOf <http://www.w3.org/2003/01/geo/wgs84_pos#SpatialThing> ;
               rdfs:comment """Regroupe l'ensemble des établissements.
Les établissements sont des lieux qui peuvent être assignés à une adresse."""@fr .


###  http://www.semanticweb.org/thoma/ontologies/2020/10/untitled-ontology-19#EtablissementSante
:EtablissementSante rdf:type owl:Class ;
                    rdfs:subClassOf :Etablissement ;
                    rdfs:comment "Regroupe l'ensemble des établissements de santé de la Réunion."@fr .


###  http://www.semanticweb.org/thoma/ontologies/2020/10/untitled-ontology-19#Laboratoires_de_Biologie_Medicale
:Laboratoires_de_Biologie_Medicale rdf:type owl:Class ;
                                   rdfs:subClassOf :EtablissementSante ;
                                   rdfs:comment "Regroupe les laboratoires de biologie médicales de l'île de la Réunion."@fr .


###  http://www.semanticweb.org/thoma/ontologies/2020/10/untitled-ontology-19#LieuRemarquable
:LieuRemarquable rdf:type owl:Class ;
                 rdfs:subClassOf :LieuTourisme ;
                 rdfs:comment """Regroupe l'ensembles des lieux dits \"remarquables\".
Il peut s'agir de forêts, de mosquées, de plages, de mares, etc."""@fr .


###  http://www.semanticweb.org/thoma/ontologies/2020/10/untitled-ontology-19#LieuTourisme
:LieuTourisme rdf:type owl:Class ;
              rdfs:subClassOf <http://www.w3.org/2003/01/geo/wgs84_pos#SpatialThing> ;
              rdfs:comment """Regroupe l'ensemble des éléments ayant un intérêt touristique.
Il peut s'agir de randonnées, de plages, de volcans, ..."""@fr .


###  http://www.semanticweb.org/thoma/ontologies/2020/10/untitled-ontology-19#Randonnee
:Randonnee rdf:type owl:Class ;
           rdfs:subClassOf :LieuTourisme ;
           rdfs:comment "Regroupe l'ensemble des circuits de randonnée de la Réunion."@fr .


###  http://www.semanticweb.org/thoma/ontologies/2020/10/untitled-ontology-19#StopCarJaune
:StopCarJaune rdf:type owl:Class ;
              rdfs:subClassOf :ArretTransport ;
              rdfs:comment "Regroupe les arrêts de car jaune de l'Ile de la Réunion."@fr .


###  http://www.semanticweb.org/thoma/ontologies/2020/10/untitled-ontology-19#Etablissements_d'Hebergement_pour_Personnes_Âgees
<http://www.semanticweb.org/thoma/ontologies/2020/10/untitled-ontology-19#Etablissements_d'Hebergement_pour_Personnes_Âgees> rdf:type owl:Class ;
                                                                                                                             rdfs:subClassOf :EtablissementSante ;
                                                                                                                             rdfs:comment "Regroupe l'ensemble des Ehpad de l'ile de la Réunion."@fr .


###  http://www.w3.org/2003/01/geo/wgs84_pos#SpatialThing
<http://www.w3.org/2003/01/geo/wgs84_pos#SpatialThing> rdf:type owl:Class ;
                                                       rdfs:comment "Regroupe l'ensemble des éléments que l'on peut placer sur une carte."@fr ;
                                                       rdfs:label "SpatialThing" .


#################################################################
#    Annotations
#################################################################

owl:Thing rdfs:comment "Regroupe l'ensemble des choses."@fr .


<http://www.w3.org/2003/01/geo/wgs84_pos#> <http://purl.org/dc/elements/1.1/date> "$Date: 2009/04/20 15:00:30 $" ;
                                           rdfs:label "geo" ;
                                           <http://purl.org/dc/elements/1.1/description> """A vocabulary for representing latitude, longitude and 
 altitude information in the WGS84 geodetic reference datum. 
 Version $Id: wgs84_pos.rdf,v 1.22 2009/04/20 15:00:30 timbl Exp $. See http://www.w3.org/2003/01/geo/ for more details.""" ;
                                           rdfs:comment """
Recent changes to this namespace:
$Log: wgs84_pos.rdf,v $
Revision 1.22  2009/04/20 15:00:30  timbl
Remove the time bits which have been deal with elsewhere eg in iCal.

Revision 1.21  2009/04/20 12:52:47  timbl
try again

Revision 1.20  2009/04/20 12:42:11  timbl
Add Event (edited ages ago and never checked in), and location (following discussion http://chatlogs.planetrdf.com/swig/2009-04-20#T12-36-09)

Revision 1.19  2009/04/20 12:36:31  timbl
Add Event (edited ages ago and never checked in), and location (following discussion http://chatlogs.planetrdf.com/swig/2009-04-20#T12-36-09)

Revision 1.18  2006/02/01 22:01:04  danbri
Clarified that lat and long are decimal degrees, and that alt is decimal metres about local reference ellipsoid

Revision 1.17  2004/02/06 17:38:12  danbri
Fixed a bad commit screwup

Revision 1.15  2003/04/19 11:24:08  danbri
Fixed the typo even more.

Revision 1.14  2003/04/19 11:16:56  danbri
fixed a typo

Revision 1.13  2003/02/19 22:27:27  connolly
relaxed domain constraints on lat/long/alt from Point to SpatialThing

Revision 1.12  2003/01/12 01:41:41  danbri
Trying local copy of XSLT doc.

Revision 1.11  2003/01/12 01:20:18  danbri
added a link to morten's xslt rdfs viewer.

Revision 1.10  2003/01/11 18:56:49  danbri
Removed datatype range from lat and long properties, since they would
have required each occurance of the property to mention the datatype.

Revision 1.9  2003/01/11 11:41:31  danbri
Another typo; repaired rdfs:Property to rdf:Property x4

Revision 1.8  2003/01/11 11:05:02  danbri
Added an rdfs:range for each lat/long/alt property,
http://www.w3.org/2001/XMLSchema#float

Revision 1.7  2003/01/10 20:25:16  danbri
Longer rdfs:comment for Point, trying to be Earth-centric and neutral about
coordinate system(s) at the same time. Feedback welcomed.

Revision 1.6  2003/01/10 20:18:30  danbri
Added CVS log comments into the RDF/XML as an rdfs:comment property of the
vocabulary. Note that this is not common practice (but seems both harmless
and potentially useful).


revision 1.5
date: 2003/01/10 20:14:31;  author: danbri;  state: Exp;  lines: +16 -5
Updated schema:
Added a dc:date, added url for more info. Changed the rdfs:label of the
namespace from gp to geo. Added a class Point, set as the rdfs:domain of
each property. Added XML comment on the lat_long property suggesting that
we might not need it (based on #rdfig commentary from implementors).

revision 1.4
date: 2003/01/10 20:01:07;  author: danbri;  state: Exp;  lines: +6 -5
Fixed typo; several rdfs:about attributes are now rdf:about. Thanks to MortenF in
#rdfig for catching this error.

revision 1.3
date: 2003/01/10 11:59:03;  author: danbri;  state: Exp;  lines: +4 -3
fixed buglet in vocab, added more wgs links

revision 1.2
date: 2003/01/10 11:01:11;  author: danbri;  state: Exp;  lines: +4 -4
Removed alt from the as-a-flat-string property, and switched from
space separated to comma separated.

revision 1.1
date: 2003/01/10 10:53:23;  author: danbri;  state: Exp;
basic geo vocab

""" ;
                                           <http://purl.org/dc/elements/1.1/title> "WGS84 Geo Positioning: an RDF vocabulary" .


<http://www.w3.org/2003/01/geo/wgs84_pos#lat_long> rdfs:comment "A comma-separated representation of a latitude, longitude coordinate." ;
                                                   rdfs:label "lat/long" .


###  Generated by the OWL API (version 4.5.9.2019-02-01T07:24:44Z) https://github.com/owlcs/owlapi
